DynamoDbEncryptionMiddlewareInternal/src/TransactWriteItemsTransform.dfy
@@ -13,15 +13,10 @@ module TransactWriteItemsTransform {
   import Seq
 
   predicate method {:opaque} IsValid(item : DDB.TransactWriteItem) {
-    item.Put.Some? || item.Update.Some? || item.Delete.Some? || item.ConditionCheck.Some?
-  }
-
-  predicate {:opaque} IsValidTransform(oldItem : DDB.TransactWriteItem, newItem : DDB.TransactWriteItem, config : map<string, ValidTableConfig>) {
-    && oldItem.ConditionCheck == newItem.ConditionCheck
-    && oldItem.Delete == newItem.Delete
-    && oldItem.Update == newItem.Update
-    && (oldItem.Put.None? ==> oldItem.Put == newItem.Put)
-    && (oldItem.Put.Some? && oldItem.Put.value.TableName !in config ==> oldItem.Put == newItem.Put)
+    || item.Put.Some?
+    || item.Update.Some?
+    || item.Delete.Some?
+    || item.ConditionCheck.Some?
   }
 
   method {:vcs_split_on_every_assert} Input(config: Config, input: TransactWriteItemsInputTransformInput)
@@ -44,30 +39,12 @@ module TransactWriteItemsTransform {
     //= specification/dynamodb-encryption-client/ddb-sdk-integration.md#encrypt-before-transactwriteitems
     //# Any `Put` actions  with a `TableName` that does not refer to an [encrypted-table](#encrypted-table),
     //# MUST be unchanged.
-    // The below has inexplicably become too difficult for Dafny
-    /*
-    ensures output.Success? ==>
-      && var result := output.value.transformedInput.TransactItems;
-      && forall i : nat | 0 <= i < |result| ::
-        && var item := input.sdkInput.TransactItems[i];
-        && item.ConditionCheck == result[i].ConditionCheck
-        && item.Delete == result[i].Delete
-        && item.Update == result[i].Update
-        && (item.Put.None? ==> item.Put == result[i].Put)
-        && (item.Put.Some? && item.Put.value.TableName !in config.tableEncryptionConfigs ==> item.Put == result[i].Put)
-        */
+    // Had a proof, but it has inexplicably become too difficult for Dafny
   {
     :- Need(forall item <- input.sdkInput.TransactItems :: IsValid(item), E("Each item in TransactWriteItems must specify at least one operation"));
     var result : seq<DDB.TransactWriteItem> := [];
     for x := 0 to |input.sdkInput.TransactItems|
       invariant |result| == x
-      // invariant forall i : nat | 0 <= i < |result| ::
-      //   && var item := input.sdkInput.TransactItems[i];
-        // && item.ConditionCheck == result[i].ConditionCheck
-        // && item.Delete == result[i].Delete
-        // && item.Update == result[i].Update
-        // && (item.Put.None? ==> item.Put == result[i].Put)
-        // && (item.Put.Some? && item.Put.value.TableName !in config.tableEncryptionConfigs ==> item.Put == result[i].Put)
     {
       var item := input.sdkInput.TransactItems[x];
 
@@ -140,8 +117,7 @@ module TransactWriteItemsTransform {
         //# the result [Encrypted DynamoDB Item](./encrypt-item.md#encrypted-dynamodb-item)
         //# calculated above.
         var put := Some(item.Put.value.(Item := encrypted.encryptedItem));
-        var newItem := item.(Put := put);
-        result := result + [newItem];
+        result := result + [item.(Put := put)];
       } else {
         result := result + [item];
       }
